
$$
\begin{gathered}
\text{证明对任何}x\geqslant0,\text{ 都有} \\
0\leqslant e^x-\sum_{k=0}^n\frac{x^k}{k!}\leqslant\frac xn(e^x-1),\forall x\in\mathbb{R},n\in\mathbb{R}\color{red}{\begin{pmatrix}1\end{pmatrix}} 
\end{gathered}
$$
注意到由 Taylor 级数，我们知道

$e^{x}=\sum_{k=0}^{\infty}\frac{x^{k}}{k!}\geqslant\sum_{k=0}^{n}\frac{x^{k}}{k!},\forall n\in\mathbb{N}.$ 
这就证明了式 (1). 此外，考虑 $f(x)=e^x-\sum_{k=0}^n\frac{x^k}{k!}-\frac xn(e^x-1)$,于是
$f'(x)=e^x-\sum_{k=1}^n\frac{x^{k-1}}{(k-1)!}-\frac{(x+1)}{n}e^x-\frac{1}{n}.$ $f^{\prime\prime}(x)=e^{x}-\sum_{k=2}^{n}\frac{x^{k-2}}{(k-2)!}-\frac{(x+2)}{n}e^{x}.$

$f^{(n)}(x)=e^{x}-1-\frac{(x+n)}{n}e^{x}.$
注意到
$f^{(n)}(x)=e^x-1-\frac{(x+n)}ne^x=-\frac{xe^x}n-1<0,f^{(j)}(0)=-\frac jn\leqslant0,j=0,1,2,\cdots,n.$ 于是显然推出对每个 $j\in\mathbb{N}$,都有 $f^{(j)}(x)$ 单调递减，于是 $f(x)\leqslant f(0)=0,\forall x\geqslant0$,这就证明了不等式(1).

