设 $f(x)$ 在$[0,1]$上非负连续且 $f(1)=0$,证明： 存在 $u\in(0,1)$ 使得 $\int_0^uf(x)dx=f(u).$


$$
\begin{aligned}&\text{令}g(x)=e^{-x}\int_0^xf(t)dt\text{则}g(0)=0,g^{\prime}(x)=e^{-x}\left(f(x)-\int_0^xf(t)dt\right)\text{是连续函数,只需证明}\\&\text{存在}u\in(0,1)\text{使得}g^{\prime}(u)=0\end{aligned}
$$
 反证法，若任意 $x\in(0,1)$ 都有 $g^{\prime}(x)\neq0$,则 $g^{\prime}(1)\neq0$,否则 $f(1)=\int_0^1f(x)dx=0$,结合 $f(x)$ 非负连续知 $f(x)=0,\forall x\in(0,1)$,则 $g(x)=0$,与 $g^{\prime}(x)\neq0$ 矛盾

 因此 $g^{\prime}(x)\geq0,\forall x\in[0,1]$,或者 $g^{\prime}(x)\leq0,\forall x\in[0,1]$,而如果后者成立，则 $g(x)$ 递减，故
 $g(x)\leq g(0)=0$,但是 $f(x)\geq0$ 且连续，所以 $f(x)=0,\forall x\in[0,1]$,则 $g(x)=0$,与 $g^{\prime}(x)\neq0$
 矛盾
 这说明 $g^{\prime}(x)\geq0,\forall x\in[0,1]$
 因为 $\int_0^xf(t)dt=e^xg(x)$,求导知 $f(x)=e^x(g(x)+g^{\prime}(x))$,由于 $f(1)=0$,所以
 $g(1)+g^{\prime}(1)=0$,由于 $f(x)$ 非负，所以 $g(1)\geq0$,由前面知 $g^{\prime}(1)\geq0$,而已经证明 $g^{\prime}(1)\neq0$
 故 $g^{\prime}(1)>0$,这与 $g(1)+g^{\prime}(1)=0$ 矛盾
 综上，我们证明了存在 $u\in(0,1)$ 使得 $g^{\prime}(u)=0$, 也就证明了本题
