
$$\begin{aligned}
&2127.\int\frac{x^2\mathrm{d}x}{(1-x^2)^3} \\
&\text{设 }y=\sqrt{1-x^2}\Rightarrow y^2+x^2=1 \\
&\int\frac{x^2\mathrm{d}x}{(1-x^2)^3}=\int\frac{1-y^2}{y^6}\mathrm{d}x=\int\frac{\mathrm{d}x}{y^6}-\int\frac{\mathrm{d}x}{y^4} \\
&\text{接下来用双元递推式即可。} \\
&\int\frac{x^2\mathrm{d}x}{(1-x^2)^3}&& =\int\frac{\mathrm{d}x}{y^6}-\int\frac{\mathrm{d}x}{y^4}  \\
&&&=\frac14\cdot\frac x{y^4}-\frac14\int\frac{\mathrm{d}x}{y^4} \\
&&&=\frac14\cdot\frac x{y^4}-\frac18\cdot\frac x{y^2}-\frac18\int\frac{\mathrm{d}x}{1-x^2} \\
&&&=\frac x{4(1-x^2)^2}-\frac x{8(1-x^2)}-\frac18\mathrm{tanh}^{-1}x
\end{aligned}$$
