
$$
\begin{aligned}
&\int_0^{+\infty}\mathrm{e}^{-x}\ln x\mathrm{d}x \\
&=\int_0^1\mathrm{e}^{-x}\ln x\mathrm{d}x+\int_1^{+\infty}\mathrm{e}^{-x}\ln x\mathrm{d}x \\
&=\int_0^1\frac{\mathrm{e}^{-x}-1}x\mathrm{d}x+\int_1^{+\infty}\frac{\mathrm{e}^{-x}}x\mathrm{d}x \\
&=\lim_{n\to\infty}\left(\int_0^n\frac{\mathrm{e}^{-x}-1}x\mathrm{d}x+\int_1^n\frac1x\mathrm{d}x\right) \\
&=\lim_{n\to\infty}\left(\int_0^n\frac{\left(1-\frac xn\right)^n-1}x\mathrm{d}x+\int_1^n\frac1x\mathrm{d}x\right) \\
&=\lim\limits_{n\to\infty}\left(-n\int_0^n\frac{\left(1-\frac{x}{n}\right)^n-1}{x}\mathrm{d}\left(1-\frac{x}{n}\right)+\ln n\right)
\end{aligned}
$$
$$
\begin{aligned}&=\lim_{n\to\infty}\left(-\int_0^1\frac{x^n-1}{x-1}\mathrm{d}x+\ln n\right)\\&=\lim_{n\to\infty}\left(-\int_0^1\left(1+x+x^2+......+x^{n-1}\right)\mathrm{d}x+\ln n\right)\\&=\lim_{n\to\infty}\left(-1-\frac12-\frac13-......-\frac1n+\ln n\right)\\&=-\gamma\end{aligned}
$$
我們可以類似推出更具有一般性的結果 $e^{-nx}\ln xdx=-\frac{\gamma+\ln n}n$
 
 