引理：
$$\begin{aligned}&\text{若}a_n=1+\frac{a}{n}+\frac{b}{n^2}+o\bigg(\frac{1}{n^2}\bigg),\text{则有如下}\\&a_n^n=e^a+\frac{e^a\bigg(b-\frac{a^2}{2}\bigg)}{n}+o\bigg(\frac{1}{n}\bigg)\\&\text{即}\lim_{n\to\infty}n\left(a_n^n-e^a\right)=e^a\bigg(b-\frac{a^2}{2}\bigg)\end{aligned}$$

证明：
 $$\begin{aligned}
&\operatorname*{lim}_{n\to\infty}a_{n}^{n}=\operatorname*{lim}_{n\to\infty}e^{n\ln a_{n}}=\operatorname*{lim}_{n\to\infty}e^{n\ln\left(1+\frac{a}{n}+\frac{b}{n^{2}}+o\left(\frac{1}{n^{2}}\right)\right)}=e^{a} \\
&\left.\lim_{n\to\infty}n\left(a_n^n-e^a\right.\right)=\lim_{n\to\infty}n\left(e^{n\ln\left(1+\frac an+\frac b{n^2}+o\left(\frac1{n^2}\right)\right)}-e^a\right) \\
&=\lim_{n\to\infty}e^an\Bigg(e^{n\ln\left(1+\frac an+\frac b{n^2}+o\left(\frac1{n^2}\right)\right)-a}-1\Bigg) \\
&=\lim_{n\to\infty}e^{a}n\Bigg[n\ln[1+\frac{a}{n}+\frac{b}{n^{2}}+o\Bigg(\frac{1}{n^{2}}\Bigg)]-a\Bigg] \\
&=\lim_{n\to\infty}e^{a}[n^{2}\ln[1+\frac{a}{n}+\frac{b}{n^{2}}+o\left(\frac{1}{n^{2}}\right)]-an] \\
&=\lim_{n\to\infty}e^a[n^2\Bigg[\frac{a}{n}+\frac{b}{n^2}+o\Bigg(\frac{1}{n^2}\Bigg)-\frac{1}{2}\Bigg[\frac{a}{n}+\frac{b}{n^2}+o\Bigg(\frac{1}{n^2}\Bigg)\Bigg]^2+o\Bigg(\frac{1}{n^2}\Bigg)\Bigg]-an\:] \\
&=\lim_{n\to\infty}e^{a}[n^{2}\Bigg[\frac{a}{n}+\frac{b}{n^{2}}+o\Bigg(\frac{1}{n^{2}}\Bigg)-\frac{1}{2}\Bigg[\frac{a}{n}\Bigg]^{2}+o\Bigg(\frac{1}{n^{2}}\Bigg)\Bigg]-an] \\
&=\lim_{n\to\infty}e^{a}\left[\left.b+o\left(1\right.\right)-\frac{1}{2}a^{2}\right]=e^{a}\left(b-\frac{a^{2}}{2}\right)
\end{aligned}$$

例题：

$$\begin{aligned}
&\operatorname*{lim}_{n\to\infty}n\left[\left({\frac{1}{\pi}}\sum_{k=1}^{n}\sin{\frac{\pi}{\sqrt{n^{2}+k}}}\right)^{n}-{\frac{1}{\sqrt[4]{e}}}\right] \\
&a_{n}={\frac{1}{\pi}}\sum_{k=1}^{n}\sin{\frac{\pi}{\sqrt{n^{2}+k}}}={\frac{1}{\pi}}\sum_{k=1}^{n}\sin{\frac{\pi}{n\sqrt{1+{\frac{k}{n^{2}}}}}} \\
&a_{n}=\frac{1}{\pi}\sum_{k=1}^{n}[\frac{\pi}{n\sqrt{1+\frac{k}{n^{2}}}}-\frac{1}{6}\Bigg(\frac{\pi}{n\sqrt{1+\frac{k}{n^{2}}}}\Bigg)^{3}+O\Bigg(\frac{\pi}{n\sqrt{1+\frac{k}{n^{2}}}}\Bigg)^{5}] \\
&=o\left(\frac{1}{n^{2}}\right)+\frac{1}{\pi}\sum_{k=1}^{n}[\frac{\pi}{n\sqrt{1+\frac{k}{n^{2}}}}-\frac{1}{6}\left(\frac{\pi}{n\sqrt{1+\frac{k}{n^{2}}}}\right)^{3}] \\
&=o\biggl(\frac{1}{n^{2}}\biggr)+\sum_{k=1}^{n}[\frac{1}{n\sqrt{1+\frac{k}{n^{2}}}}-\frac{\pi^{2}}{6}\biggl(\frac{1}{n\sqrt{1+\frac{k}{n^{2}}}}\biggr)^{3}] \\
&=o\left(\frac{1}{n^{2}}\right)+\sum_{k=1}^{n}[\frac{1}{n\sqrt{1+\frac{k}{n^{2}}}}-\frac{\pi^{2}}{6}\left(\frac{1}{n\sqrt{1+\frac{k}{n^{2}}}}\right)^{3}] \\
&\frac{1}{\sqrt{1+x}}=\left(1+x\right)^{-\frac{1}{2}}=\sum_{k=0}^{\infty}C_{\frac{1}{2}}^{k}x^{k}=1-\frac{1}{2}x+\frac{3}{8}x^{2}+o\left(x^{2}\right) \\
&\text{其中}C_{a}^{k}={\frac{a\left(a-1\right)...\left(a-k+1\right)}{k!}}\text{是广义二项式系数}.
\end{aligned}$$

$$\begin{aligned}
&\text{故}& a_{n}=o\left(\frac{1}{n^{2}}\right)+\sum_{k=1}^{n}\frac{1}{n}[1-\frac{1}{2}\frac{k}{n^{2}}+\frac{3}{8}\frac{k^{2}}{n^{4}}+o\left(\frac{1}{n^{2}}\right)]-\frac{\pi^{2}}{6}\sum_{k=1}^{n}\left(\frac{1}{n\sqrt{1+\frac{k}{n^{2}}}}\right)^{3}  \\
&=o\left(\frac{1}{n^{2}}\right)+\sum_{k=1}^{n}\frac{1}{n}[1-\frac{1}{2}\frac{k}{n^{2}}+\frac{3}{8}\frac{k^{2}}{n^{4}}]-\frac{\pi^{2}}{6}\frac{1}{n^{3}}\sum_{k=1}^{n}\left(\frac{1}{\sqrt{1+\frac{k}{n^{2}}}}\right)^{3} \\
&=o\Bigg(\frac{1}{n^{2}}\Bigg)+\sum_{k=1}^{n}\frac{1}{n}[1-\frac{1}{2}\frac{k}{n^{2}}+\frac{3}{8}\frac{k^{2}}{n^{4}}]-\frac{\pi^{2}}{6}\frac{1}{n^{3}}\sum_{k=1}^{n}\Bigg(1+O\Bigg(\frac{k}{n^{2}}\Bigg)\Bigg)^{3} \\
&=o\left(\frac{1}{n^{2}}\right)+\sum_{k=1}^{n}\frac{1}{n}[1-\frac{1}{2}\frac{k}{n^{2}}+\frac{3}{8}\frac{k^{2}}{n^{4}}]-\frac{\pi^{2}}{6}\frac{1}{n^{3}}\sum_{k=1}^{n}\left(1+O\left(\frac{1}{n}\right)\right)^{3} \\
&=o\left(\frac{1}{n^{2}}\right)+\sum_{k=1}^{n}\frac{1}{n}[1-\frac{1}{2}\frac{k}{n^{2}}+\frac{3}{8}\frac{k^{2}}{n^{4}}]-\frac{\pi^{2}}{6}\frac{1}{n^{3}}\sum_{k=1}^{n}1 \\
&=o\Bigg(\frac{1}{n^{2}}\Bigg)+\sum_{k=1}^{n}\frac{1}{n}[1-\frac{1}{2}\frac{k}{n^{2}}+\frac{3}{8}\frac{k^{2}}{n^{4}}]-\frac{\pi^{2}}{6}\frac{1}{n^{2}} \\
&=o\left(\frac{1}{n^{2}}\right)+1-\frac{\left(n+1\right)}{4n^{2}}+\frac{1}{16}\frac{\left(n+1\right)\left(2n+1\right)}{n^{4}}-\frac{\pi^{2}}{6}\frac{1}{n^{2}} \\
&=o\left(\frac{1}{n^{2}}\right)+1-\frac{\left(n+1\right)}{4n^{2}}+\frac{1}{16}\frac{2\:n^{2}}{n^{4}}-\frac{\pi^{2}}{6}\frac{1}{n^{2}} \\
&=1-\frac{1}{4n}-\left(\frac{\pi^{2}}{6}+\frac{1}{8}\right)\frac{1}{n^{2}}+o\left(\frac{1}{n^{2}}\right) \\
&\text{故}\lim_{n\to\infty}a_n^n=e^{-\frac14},\lim_{n\to\infty}n(a_n^n-e^{-\frac14})=-e^{-\frac14}\left[\frac{\pi^2}{6}+\frac18+\frac1{32}\right] \\
&=-e^{-\frac{1}{4}}\left[\frac{\pi^{2}}{6}+\frac{5}{32}\right]
\end{aligned}$$
