$$\begin{aligned}&\lim_{x\to0}\frac{1-\cos x\sqrt{1-x^2}}{1+x^2-\cos^2x}\\&\left(1+x\right)^{\frac12}=1+\frac x2+O\left(x^2\right)\\&\sqrt{1-x^2}=1-\frac{x^2}2+O\left(x^4\right)\\&\cos^2x=1-x^2+O\left(x^4\right)\\&\cos x=1-\frac{x^2}2+O\left(x^4\right)\end{aligned}$$

其中，我们对于我们的 $\sqrt{ 1-x^{2} }$ 的展开就利用到了我们的二项式公式。于是，我们就可以得到我们的下面的答案：
$$\lim_{x\to0}\frac{1-\cos x\sqrt{1-x^2}}{1+x^2-\cos^2x}=\lim_{x\to0}\frac{1-\left(1-\frac{x^2}{2}+O\left(x^4\right)\right)\left(1-\frac{x^2}{2}+O\left(x^4\right)\right)}{1+x^2-\left(1-x^2+O\left(x^4\right)\right)}$$
$$1-\left(1-\frac{x^2}2\right)^2+O\left(x^4\right)\\=\lim_{x\to0}\frac{1-\left(1-\frac{x^2}2\right)^2+O\left(x^4\right)}{2x^2+O\left(x^4\right)}=\lim_{x\to0}\frac{\frac{x^2}2\left(2-\frac{x^2}2\right)+O\left(x^4\right)}{2x^2+O\left(x^4\right)}$$
$$=\lim_{x\to0}\frac{x^2+O\Big(x^4\Big)}{2x^2+O\Big(x^4\Big)}=\lim_{x\to0}\frac{1+\frac{O\Big(x^4\Big)}{x^2}}{2+\frac{O\Big(x^4\Big)}{x^2}}=\frac12$$