
$$
I=\lim_{x\to0^+}\frac{x^{(\sin x)^x}-(\sin x)^{x^{\sin x}}}{x^3}.
$$


$$=\lim_{x\to0^+}\frac{e^{\left(x-\frac{x^3}6+o(x^3)\right)^x\ln x}-e^{x^{\left(x-\frac{x^3}6+o\left(x^3\right)\right)}\ln\left(x-\frac{x^3}6+o\left(x^3\right)\right)}}{x^3}$$
$$
\begin{aligned}
&=\lim_{x\to0^+}\frac{e^{x^{\left(x-\frac{x^3}6\right)}\ln\left(x-\frac{x^3}6\right)}}x*\lim_{x\to0^+}\frac{e^{\left(x-\frac{x^3}6\right)^x\ln x-x^{\left(x-\frac{x^3}6\right)}\ln\left(x-\frac{x^3}6\right)}-1}{x^2} \\
&=1*\lim_{x\to0^+}\frac{\left(x-\frac{x^3}6\right)^x\ln x-x^{\left(x-\frac{x^3}6\right)}\ln\left(x-\frac{x^3}6\right)}{x^2} \\
&=\lim_{x\to0^+}\frac{\left[\left(x-\frac{x^3}6\right)^x-x^{\left(x-\frac{x^3}6\right)}\right]\ln x}{x^2}-\lim_{x\to0^+}\frac{x^{\left(x-\frac{x^3}6\right)}\left(-\frac{x^2}6\right)}{x^2} \\
&=0-\left(-\frac16\right)=\frac16
\end{aligned}
$$
