
$$\begin{aligned}
&\lim_{n\to\infty}\frac{\sum_{k=0}^n\ln C_n^k}{n^2} \\
&\begin{aligned}=\lim_{n\to\infty}\frac{\sum_{k=0}^{n+1}\ln C_{n+1}^k-\sum_{k=0}^n\ln C_n^k}{\left(n+1\right)^2-n^2}&=\lim_{n\to\infty}\frac{\sum_{k=0}^{n+1}\ln C_{n+1}^k-\sum_{k=0}^n\ln C_n^k}{2n+1}\end{aligned} \\
&=\lim_{n\to\infty}\frac{\sum_{k=0}^n\ln C_{n+1}^k-\sum_{k=0}^n\ln C_{n}^k}{2n+1}=\lim_{n\to\infty}\frac{\sum_{k=1}^n\ln C_{n+1}^k-\sum_{k=1}^n\ln C_{n}^k}{2n+1} \\
&=\lim_{n\to\infty}\frac{\sum_{k=1}^n\ln\left[\frac{n+1}kC_n^{k-1}\right]-\sum_{k=1}^n\ln C_n^k}{2n+1}=\lim_{n\to\infty}\frac{\sum_{k=1}^n[\ln\left(n+1\right)-\ln k]+\sum_{k=1}^n\ln C_n^{k-1}-\sum_{k=1}^n\ln C_n^k}{2n} \\
&=\lim_{n\to\infty}\frac{\sum_{k=1}^n[\ln\left(n+1\right)-\ln k]}{2n}=\lim_{n\to\infty}\frac{n\ln\left(n+1\right)-\sum_{k=1}^n\ln k}{2n} \\
&=\lim_{n\to\infty}\frac{\left(n+1\right)\ln\left(n+2\right)-n\ln\left(n+1\right)-\ln\left(n+1\right)}2 \\
&=\lim_{n\to\infty}\frac{n\ln[\frac{n+2}{n+1}]}{2}=\frac12 \\
&=\lim_{n\to\infty}\frac{\sum_{k=0}^n\ln C_n^k}{n^2}
\end{aligned}$$


$$\begin{aligned}
&\lim_{n\to\infty}\frac{\ln n}{\ln\sum_{k=1}^{n}k^{2020}} \\
&=\lim_{n\to\infty}\frac{\ln(n+1)-\ln n}{\ln\sum_{k=1}^{n+1}k^{2020}-\ln\sum_{k=1}^nk^{2020}}=\lim_{n\to\infty}\frac{\ln(1+\frac1n)}{\ln\sum_{k=1}^{n+1}k^{2020}-\ln\sum_{k=1}^nk^{2020}} \\
&=\lim_{n\to\infty}\frac{\frac1n}{\sum_{k=1}^{n+1}k^{2020}}=\lim_{n\to\infty}\frac{\frac1n}{\ln\left(1+\frac{\left(n+1\right)^{2020}}{\sum_{k=1}^{n}k^{2020}}\right)}=\lim_{n\to\infty}\frac1{n\frac{\left(n+1\right)^{2020}}{\sum_{k=1}^{n}k^{2020}}} \\
&=\lim_{n\to\infty}\frac{\sum_{k=1}^{n}k^{2020}}{n\left(n+1\right)^{2020}}=\lim_{n\to\infty}\frac{\sum_{k=1}^{n}k^{2020}}{n^{2021}}=\lim_{n\to\infty}\int_{0}^{1}x^{2020}dx=\frac{1}{2021}
\end{aligned}$$
