六、(本题 14 分) 设数列 $\{x_n\}$ 满足 $x_{0}=\frac{1}{3}$,
$x_{n+1}=\frac{x_{n}^{2}}{1-x_{n}+x_{n}^{2}},n\geqslant0$.证明：无穷级数 $\sum x_n$ 收敛并求其
和

方法 1. 根据数学归纳法可知 $x_n>0.$ 此外，$x_{n+1}-x_{n}=-\frac{x_{n}(1-x_{n})^{2}}{1-x_{n}+x_{n}^{2}}<0.$
 故 $x_n$ 单调递减，$x_n\leqslant\frac13.$
 于是，$x_{n+1}=x_n\cdot\frac{x_n}{1-x_n+x_n^2}\leqslant\frac{4}{9}x_n$,

 令 $f(x)=\frac{x}{1+x},x>0$, 不难验证 $f(x)$ ) $^{\mathrm{uz}}$ 格单调递增且其反函数为 $f^{-1}(x)=\frac{x}{1-x}.$
 注意到 $x_{n+1}=f(f^{-1}(x_n)-x_n)$,故

$$
\begin{aligned}f^{-1}(x_{n+1})&=f^{-1}(x_n)-x_n,\quad x_n=f^{-1}(x_n)-f^{-1}(x_{n+1}).\\\sum_{i=0}^nx_i&=f^{-1}(x_0)-f^{-1}(x_{n+1}).\end{aligned}
$$

$$
\sum_{i=0}^{\infty}x_{i}=f^{-1}(x_{0})-f^{-1}(0)=\frac{1}{2}.
$$


## 方法二：裂项：
$$\begin{aligned}&\because\quad x_{n+1}=\frac{x_{n}^{2}}{1-x_{n}+x_{n}^{2}},\quad x_{n+1}(1-x_{n}+x_{n}^{2})=x_{n}^{2},\\&x_{n+1}\left(1-x_{n}\right)+x_{n}^{2}x_{n+1}=x_{n}^{2},\quad x_{n+1}\left(1-x_{n}\right)=x_{n}^{2}\left(1-x_{n+1}\right),\\&\frac{x_{n}^{2}}{1-x_{n}}=\frac{x_{n+1}}{1-x_{n+1}},\quad\frac{x_{n}^{2}-x_{n}+x_{n}}{1-x_{n}}=\frac{x_{n+1}}{1-x_{n+1}},\\&\frac{x_{n}-x_{n}\left(1-x_{n}\right)}{1-x_{n}}=\frac{x_{n+1}}{1-x_{n+1}},\quad\frac{x_{n}}{1-x_{n}}-\frac{x_{n}\left(1-x_{n}\right)}{1-x_{n}}=\frac{x_{n+1}}{1-x_{n+1}},\\&\frac{x_{n}}{1-x_{n}}-x_{n}=\frac{x_{n+1}}{1-x_{n+1}},\quad\therefore\quad x_{n}=\frac{x_{n}}{1-x_{n}}-\frac{x_{n+1}}{1-x_{n+1}}\text{知乎@人生}\end{aligned}$$
