
$f\big(x\big)\in C^{1}\big(0,+\infty\big)$

$$\lim\limits_{x\to+\infty}f’\left(x\right)+f\left(x\right)=a,\text{计算}\lim\limits_{x\to+\infty}f\left(x\right)$$

$$
\lim_{x\to+\infty}f’\left(x\right)+\frac{2x}{\sqrt[3]{1+x^3}}f\left(x\right)=a,\:\text{计算}\lim_{x\to+\infty}f\left(x\right)
$$


$$\begin{aligned}
&\operatorname*{lim}_{x\to+\infty}f\left(x\right)=\operatorname*{lim}_{x\to+\infty}\frac{e^{x}f\left(x\right)}{e^{x}}=\operatorname*{lim}_{x\to+\infty}\frac{e^{x}\left[f\left(x\right)+f^{-\prime}\left(x\right)\right]}{e^{x}}=\operatorname*{lim}_{x\to+\infty}f^{-\prime}\left(x\:\right)+f\:\left(x\:\right)=a \\
&\lim_{x\to+\infty}f\left(x\right)=\lim_{x\to+\infty}\frac{g\left(x\right)f\left(x\right)}{g\left(x\right)} \\
&=\lim_{x\to+\infty}\frac{g’\left(x\right)f\left(x\right)+g\left(x\right)f’\left(x\right)}{g’\left(x\right)}=\lim_{x\to+\infty}f\left(x\right)+\frac{g\left(x\right)}{g’\left(x\right)}f’\left(x\right) \\
&\lim_{x\to+\infty}f’\left(x\right)+\frac{2x}{\sqrt[3]{1+x^{3}}}f\left(x\right)=2\lim_{x\to+\infty}\frac{\sqrt[3]{1+x^{3}}}{2x}f’\left(x\right)+f\left(x\right)=\lim_{x\to+\infty}2a\:\frac{\sqrt[3]{1+x^{3}}}{2x}=a \\
&\textit{凑}\frac{g\left(x\right)}{g’\left(x\right)}=\frac{\sqrt[3]{1+x^3}}{2x}\Rightarrow\left[\ln g\left(x\right)\right]’=\frac{g’\left(x\right)}{g\left(x\right)}=\frac{2x}{\sqrt[3]{1+x^3}}\rightarrow2
\end{aligned}$$

