例题 2.32 (上海交通大学 1991 年竞赛题) 设 $x_{1}=1,x_{2}=2$,且
$$x_{n+2}=\sqrt{x_{n+1}\cdot x_n}\:(n=1,2,\cdots)$$
求 $\lim_n\to\infty x_n$

证明令 $y_n=\ln x_n$,则由 $x_{n+2}=\sqrt{x_{n+1}\cdot x_n}$ 得 $y_{n+2}=\frac12(y_{n+1}+y_n)$,故
$y_{n+2}-y_{n+1}=-\frac{1}{2}(y_{n+1}-y_{n})=\left(-\frac{1}{2}\right)^{2}(y_{n}-y_{n-1})$

移项得

$=\cdots=\left(-\frac{1}{2}\right)^{n}(y_{2}-y_{1})=\left(-\frac{1}{2}\right)^{n}\ln2$
$y_{n+2}=y_{n+1}+\left(-\frac12\right)^n\ln2=y_n+\left(-\frac12\right)^{n-1}\ln2+\left(-\frac12\right)^n\ln2$
$=\cdots=y_{1}+\left[\left(-\frac{1}{2}\right)^{0}\ln2+\left(-\frac{1}{2}\right)\ln2+\cdots+\left(-\frac{1}{2}\right)^{n}\ln2\right]$
$=\ln2\left[1+\left(-\frac{1}{2}\right)+\left(-\frac{1}{2}\right)^{2}+\cdots+\left(-\frac{1}{2}\right)^{n}\right]$ $=\ln2\cdot\frac{1-\left(-\frac{1}{2}\right)^{n+1}}{1+\frac{1}{2}}=\frac{2}{3}\left[1-\left(-\frac{1}{2}\right)^{n+1}\right]\ln2$
故 $\lim_{n\to\infty}y_{n+2}=\frac{2}{3}\lim_{n\to\infty}\left[1-\left(-\frac{1}{2}\right)^{n+1}\right]\ln2=\frac{2}{3}\ln2$,于是
$$\lim_{n\to\infty}x_n=\lim_{n\to\infty}x_{n+2}=\lim_{n\to\infty}e^{y_{n+2}}=e^{\lim_{n\to\infty}y_{n+2}}=2^{\frac{2}{3}}$$