
$$\lim\limits_{n\to\infty}a_n-\lambda a_{n-1}=a,\left|\lambda\right|<1,\text{计算}\lim\limits_{n\to\infty}a_n$$

$$\begin{aligned}
&\text{证明:} \\
&\lambda=0,\text{显然,}\lambda\neq0\text{时} \\
&b_{n}=a_{n}-\lambda a_{n-1},\operatorname*{lim}_{n\to\infty}b_{n}=a,\:\text{视为}b_{n}\text{已知},\:\text{强求}a_{n}\:\text{通项}: \\
&\frac{a_{n}}{\lambda^{n}}-\frac{a_{n-1}}{\lambda^{n-1}}=\frac{b_{n}}{\lambda^{n}},\frac{a_{n}}{\lambda^{n}}-a_{0}=\sum_{k=1}^{n}\frac{b_{k}}{\lambda^{k}} \\
&a_{n}=\lambda^{n}a_{0}+\lambda^{n}\sum_{k=1}^{n}\frac{b_{k}}{\lambda^{k}} \\
&\operatorname*{lim}_{n\to\infty}\lambda^{n}\sum_{k=1}^{n}\frac{b_{k}}{\lambda^{k}},\text{不妨设}\lambda>0, \\
&\text{当}\lambda<0\text{虽然多个符号},\text{但是可以分奇偶类似操作},\text{留作习题}. \\
&\lim_{n\to\infty}\frac{\sum_{k=1}^n\frac{b_k}{\lambda^k}}1=\lim_{n\to\infty}\frac{\frac{b_{n+1}}{\lambda^{n+1}}}{1}=\frac a{1-\lambda}
\end{aligned}$$
