已知微分方程 $y^{\prime}=1+x(y-y^{\prime\prime})$ 的解 $y$ 满足 $y(0)=\frac\pi2,y^{\prime}(0)=1,y^{\prime\prime}(0)=\frac\pi4$,计算 $\int_0^1y(x)dx.$


## 解

$$
y(x)=\sum_{n=0}^\infty a_nx^n,y^{\prime}(x)=\sum_{n=1}^\infty na_nx^{n-1},y^{\prime\prime}(x)=\sum_{n=2}^\infty n(n-1)a_nx^{n-2}.
$$

$$
\sum_{n=1}^\infty na_nx^{n-1}=1+\sum_{n=0}^\infty a_nx^{n+1}-\sum_{n=2}^\infty n(n-1)a_nx^{n-1},
$$

$$
\sum_{n=0}^\infty(n+2)a_{n+2}x^{n+1}=\sum_{n=0}^\infty a_nx^{n+1}-\sum_{n=0}^\infty(n+2)(n+1)a_{n+2}x^{n+1}.
$$

$$
(n+2)a_{n+2}=a_n-(n+2)(n+1)a_{n+2},n=0,1,2,\cdots 
$$

$$
a_{n+2}=\frac{1}{\left(n+2\right)^{2}}a_{n},n=0,1,2,\cdots.
$$

$$
a_{2n}=\frac{1}{\left[(2n)!!\right]^{2}}\frac{\pi}{2},a_{2n+1}=\frac{1}{\left[(2n+1)!!\right]^{2}},n=0,1,2,\cdots,
$$

$$
\begin{aligned}
\int_{0}^{1}y(x)dx& =\sum_{n=0}^{\infty}\int_0^1\left(a_{2n}x^{2n}+a_{2n+1}x^{2n+1}\right)dx  \\
&=\sum_{n=0}^{\infty}\biggl(\frac{a_{2n}}{2n+1}+\frac{a_{2n+1}}{2n+2}\biggr) \\
&=\frac{\pi+1}{2}+\sum_{n=1}^{\infty}\left(\frac{\pi}{2}\frac{1}{(2n+1)[(2n)!!]^{2}}+\frac{1}{(2n+2)[(2n+1)!!]^{2}}\right) \\
&=\frac{1}{2}\left(\pi_{1}F_{2}\bigg(\frac{1}{2};1,\frac{3}{2};\frac{1}{4}\bigg)+_{2}F_{3}\bigg(1,1;\frac{3}{2},\frac{3}{2},2;\frac{1}{4}\bigg)\bigg)\approx2.2352,\right. 
\end{aligned}
$$

